refactor!: Change MultiKeyring.children to a seq<Keyring> (#223)

src/extern/dotnet/MessageHeader.cs
@@ -1,22 +1,23 @@
 using System;
 using System.Linq;
 using System.Collections.Generic;
+using ibyteseq = Dafny.ISequence<byte>;
 using byteseq = Dafny.Sequence<byte>;
 
 namespace MessageHeader {
 
   public partial class __default {
 
-    public static Dafny.Map<byteseq,byteseq> KVPairSequenceToMap(Dafny.Sequence<_System.Tuple2<byteseq,byteseq>> kvPairs) {
-        Dictionary<byteseq, byteseq> dict = kvPairs.Elements.ToDictionary(
+    public static Dafny.Map<ibyteseq,ibyteseq> KVPairSequenceToMap(Dafny.ISequence<_System.Tuple2<ibyteseq,ibyteseq>> kvPairs) {
+        Dictionary<ibyteseq, ibyteseq> dict = kvPairs.Elements.ToDictionary(
             item => item._0,
             item => item._1);
-        List<Dafny.Pair<byteseq, byteseq>> pairs = new List<Dafny.Pair<byteseq, byteseq>>();
+        List<Dafny.Pair<ibyteseq, ibyteseq>> pairs = new List<Dafny.Pair<ibyteseq, ibyteseq>>();
 
-        foreach(KeyValuePair<byteseq, byteseq> entry in dict) {
-            pairs.Add(new Dafny.Pair<byteseq, byteseq>(entry.Key, entry.Value));
+        foreach(KeyValuePair<ibyteseq, ibyteseq> entry in dict) {
+            pairs.Add(new Dafny.Pair<ibyteseq, ibyteseq>(entry.Key, entry.Value));
         }
-        return Dafny.Map<byteseq,byteseq>.FromCollection(pairs);
+        return Dafny.Map<ibyteseq,ibyteseq>.FromCollection(pairs);
     }
   }
 }
